Working in a different approach of ctx
I'll add the assumption that the environment will not be shadowed because
we only add variables that does not appear in the context.
Maybe changing the ctx to a list will be slightly better? idk

src/Coq/Metatheory.v
@@ -194,8 +194,8 @@ Notation " m 'extd' id ':' val" := (extend m id val) (at level 20, id at next le
 (* Extends a list of element at the tail of the map *)
 Fixpoint extend_list {A:Type} (m : partial_map A) (ids : list id) (vals : list A) :=
 match ids, vals with
- | (x::xs), (v::vs) => extend_list (extend m x v) xs vs
- | _, _ => m
+ | (x::xs), (v::vs) => (update (extend_list m xs vs) x v)
+ | _, _ => m 
 end.
 
 Notation " m 'extds' ids ':' vals" := (extend_list m ids vals) (at level 20, ids at next level).
@@ -242,6 +242,36 @@ Proof.
   simpl. auto.
 Qed.
 
+Lemma ex': forall A xs ds (m: partial_map A) x di,
+  (m extds (x::xs) : (di::ds)) x = Some di.
+Proof.
+  intros; simpl. unfold update. rewrite beq_id_refl; auto.
+Qed.
+
+Lemma ex: forall A xs ds i xi di (m: partial_map A),
+  nth_error xs i = Some xi ->
+  length xs = length ds ->
+  (m extds xs : ds) xi = Some di ->
+  nth_error ds i = Some di.
+Proof.
+  induction xs, ds; intros; try (solve [
+    match goal with 
+    | [ H: (nth_error [] _ = _) |- _ ] => rewrite nth_error_nil in H; inversion H 
+    end
+    ]).
+  inversion H0.
+  destruct i eqn:Heq. inversion H.
+  rewrite H3 in H1.
+  rewrite ex' in H1. simpl; auto.
+  simpl in *. inversion H0. eapply IHxs; eauto.
+ simpl in *.
+  
+   unfold extend_list in H1.
+  rewrite beq_id_refl in H1.
+  simpl in H1.
+Admitted.
+
+(*
 Lemma extend_list_not_shadow: forall A (m: partial_map A) x xs ds,
 ~In x xs ->
 (m extds xs : ds) x = m x.
@@ -257,6 +287,20 @@ Proof.
   rewrite not_eq_beq_id_false; auto.
 Qed.
 
+
+Lemma extend_list_not_shadow': forall A xs ds (m: partial_map A) x,
+Forall (fun x' => m x' = None) xs ->
+In x xs ->
+length xs = length ds ->
+(m extds xs : ds) x = (empty extds xs : ds) x.
+Proof.
+  induction xs, ds; intros; try (solve [inversion H0| inversion H1]).
+  simpl in *. inversion H1.
+  destruct eq_id_dec with a x. rewrite e. 
+ simpl. unfold empty.
+  simpl.
+*)
+
 Lemma extend_neq : forall A (m: partial_map A) v x x0,
 x <> x0 ->
 (extend m x v) x0 = m x0.
@@ -265,6 +309,7 @@ Proof.
   case (m x2). auto.
   rewrite not_eq_beq_id_false; auto.
 Qed.
+
 
 Section Ref.
 
