src/Coq/Syntax.v
@@ -120,8 +120,8 @@ Inductive m_type (m: id) (C: ClassName) (Bs: [ClassName]) (B: ClassName) : Prop:
               map fargType fargs = Bs ->
               mtype(m, D) = Bs ~> B ->
               mtype(m, C) = Bs ~> B
-  where "'mtype(' m ',' D ')' '=' c '~>' c0"
-        := (m_type m D c c0).
+  where "'mtype(' m ',' D ')' '=' cs '~>' c0"
+        := (m_type m D cs c0).
 
 
 Inductive m_body (m: id) (C: ClassName) (xs: [ClassName]) (e: Exp) : Prop:=
@@ -160,6 +160,68 @@ Notation " [; ds '\' xs ;] e " := (subst e ds xs) (at level 30).
 Eval compute in ([;(ExpVar this) :: ExpFieldAccess (ExpVar this) (Id 2) :: nil \ Id 2 :: Id 1 :: nil;] ExpVar (Id 1)).
 Check (subst (ExpVar (Id 1)) ((ExpFieldAccess (ExpVar this) (Id 2))::nil)) ((Id 1)::nil).
 
+(*
+Fixpoint subst (e: Exp) (v: Var) (e': Exp) : Exp:=
+  match e with
+  | ExpVar var => if beq_id var v then e' else e
+  | ExpFieldAccess exp i => ExpFieldAccess (subst exp v e') i
+  | ExpMethodInvoc exp i exps => 
+      ExpMethodInvoc (subst exp v e') i (map (fun x => subst x v e') exps)
+  | ExpCast cname exp => ExpCast cname (subst exp v e')
+  | ExpNew cname exps => ExpNew cname (map (fun x => subst x v e') exps)
+  end.
+Notation " ([ v' '\' v ']' e )" := (subst e v v') (at level 35).
+
+Eval compute in (([ExpFieldAccess (ExpVar this) (Id 2) \ Id 1] ExpVar (Id 1))).
+Inductive subst_list : Exp -> [Var] -> [Exp] -> Exp -> Prop :=
+  | Subst_Var : forall ds xs xi di i,
+      nth_error xs i = Some xi->
+      nth_error ds i = Some di ->
+      [; ds \ xs ;] (ExpVar xi) = di
+  | Subst_FieldAcc : forall e: Exp, [; ds \ xs ;] e = e
+  | Subst_Invk : forall e: Exp, [; nil \ nil ;] e = e
+  | Subst_Cast : forall e: Exp, [; nil \ nil ;] e = e
+  | Subst_New : forall e: Exp, [; nil \ nil ;] e = e
+  | Subst_cons : forall e1 e2 e3 (e': Exp) (v: Var) es vs,
+    ([e' \ v] e1) = e2->
+    [;es \ vs;] e2 = e3 ->
+    [; e'::es \ v::vs ;] e1 = e3
+where " [; es '\' vs ;] e1 '=' e2 " := (subst_list e1 vs es e2).
+Print ExpVar.
+*)
+
+Inductive appears_free_in : Var -> Exp -> Prop :=
+  | afi_var : forall x,
+    appears_free_in x (ExpVar x)
+  | afi_field : forall x e fi,
+    appears_free_in x e ->
+    appears_free_in x (ExpFieldAccess e fi)
+  | afi_m_invk1 : forall x e mname es,
+    appears_free_in x e ->
+    appears_free_in x (ExpMethodInvoc e mname es)
+  | afi_m_invk2 : forall x e e' mname es,
+    In e' es ->
+    appears_free_in x e' ->
+    appears_free_in x (ExpMethodInvoc e mname es)
+  | afi_cast : forall x e CName,
+    appears_free_in x e ->
+    appears_free_in x (ExpCast CName e)
+  | afi_new : forall x e es CName,
+    In e es ->
+    appears_free_in x e ->
+    appears_free_in x (ExpNew CName es).
+
+Hint Constructors appears_free_in.
+Tactic Notation "afi_cases" tactic(first) ident(c) :=
+  first;
+  [ Case_aux c "afi_var" | Case_aux c "afi_field"
+  | Case_aux c "afi_m_invk1" | Case_aux c "afi_m_invk2"
+  | Case_aux c "afi_cast" | Case_aux c "afi_new"].
+
+
+Definition closed (e: Exp) :=
+  forall x, ~ appears_free_in x e.
+
 Inductive Warning (s: string) : Prop :=
   | w_str : Warning s.
 Notation stupid_warning := (Warning "stupid warning").
@@ -178,14 +240,14 @@ Inductive ExpTyping (Gamma: partial_map ClassName) : Exp -> ClassName -> Prop :=
   | T_Invk : forall e0 C Cs C0 Ds m es,
                 Gamma |- e0 : C0 ->
                 mtype(m, C0) = Ds ~> C ->
-                Forall' (ExpTyping Gamma) es Cs ->
-                Forall' Subtype Cs Ds ->
+                Forall2 (ExpTyping Gamma) es Cs ->
+                Forall2 Subtype Cs Ds ->
                 Gamma |- ExpMethodInvoc e0 m es : C
   | T_New : forall C Ds Cs fs es,
                 fields C fs ->
                 Ds = map fieldType fs ->
-                Forall' (ExpTyping Gamma) es Cs ->
-                Forall' Subtype Cs Ds ->
+                Forall2 (ExpTyping Gamma) es Cs ->
+                Forall2 Subtype Cs Ds ->
                 Gamma |- ExpNew C es : C
   | T_UCast : forall e0 D C,
                 Gamma |- e0 : D ->
@@ -267,16 +329,16 @@ Definition ExpTyping_ind' :=
         Gamma |- e0 : C0 ->
         P e0 C0 ->
         mtype( m, C0)= Ds ~> C ->
-        Forall' (ExpTyping Gamma) es Cs ->
-        Forall' Subtype Cs Ds -> 
-        Forall' P es Cs ->
+        Forall2 (ExpTyping Gamma) es Cs ->
+        Forall2 Subtype Cs Ds -> 
+        Forall2 P es Cs ->
         P (ExpMethodInvoc e0 m es) C)
   (f2 : forall (C : id) (Ds Cs : [ClassName]) (fs : [FieldDecl]) (es : [Exp]),
         fields C fs ->
         Ds = map fieldType fs ->
-        Forall' (ExpTyping Gamma) es Cs ->
-        Forall' Subtype Cs Ds -> 
-        Forall' P es Cs ->
+        Forall2 (ExpTyping Gamma) es Cs ->
+        Forall2 Subtype Cs Ds -> 
+        Forall2 P es Cs ->
         P (ExpNew C es) C)
   (f3 : forall (e0 : Exp) (D C : ClassName), Gamma |- e0 : D -> P e0 D -> D <: C -> P (ExpCast C e0) C)
   (f4 : forall (e0 : Exp) (C : id) (D : ClassName),
@@ -289,19 +351,19 @@ fix F (e : Exp) (c : ClassName) (e0 : Gamma |- e : c) {struct e0} : P e c :=
   | T_Field _ e1 C0 fs i Fi Ci fi e2 f6 e3 e4 e5 => f0 e1 C0 fs i Fi Ci fi e2 (F e1 C0 e2) f6 e3 e4 e5
   | T_Invk _ e1 C Cs C0 Ds m es e2 m0 f6 f7 => f1 e1 C Cs C0 Ds m es e2 (F e1 C0 e2) m0 f6 f7 
           ((fix list_Forall_ind (es' : [Exp]) (Cs' : [ClassName]) 
-            (map : Forall' (ExpTyping Gamma) es' Cs'): 
-               Forall' P es' Cs' :=
+            (map : Forall2 (ExpTyping Gamma) es' Cs'): 
+               Forall2 P es' Cs' :=
             match map with
-            | Forall'_nil _ _ _ => Forall'_nil Exp ClassName P
-            | Forall'_cons _ _ _ ex cx ees css H1 H2 => Forall'_cons Exp ClassName P ex cx ees css (F ex cx H1) (list_Forall_ind ees css H2)
+            | Forall2_nil _ => Forall2_nil P
+            | (@Forall2_cons _ _ _ ex cx ees ccs H1 H2) => Forall2_cons ex cx (F ex cx H1) (list_Forall_ind ees ccs H2)
           end) es Cs f6)
   | T_New _ C Ds Cs fs es f6 e1 f7 f8 => f2 C Ds Cs fs es f6 e1 f7 f8
           ((fix list_Forall_ind (es' : [Exp]) (Cs' : [ClassName]) 
-            (map : Forall' (ExpTyping Gamma) es' Cs'): 
-               Forall' P es' Cs' :=
+            (map : Forall2 (ExpTyping Gamma) es' Cs'): 
+               Forall2 P es' Cs' :=
             match map with
-            | Forall'_nil _ _ _ => Forall'_nil Exp ClassName P
-            | Forall'_cons _ _ _ ex cx ees css H1 H2 => Forall'_cons Exp ClassName P ex cx ees css (F ex cx H1) (list_Forall_ind ees css H2)
+            | Forall2_nil _ => Forall2_nil P
+            | (@Forall2_cons _ _ _ ex cx ees ccs H1 H2) => Forall2_cons ex cx (F ex cx H1) (list_Forall_ind ees ccs H2)
           end) es Cs f7)
   | T_UCast _ e1 D C e2 s => f3 e1 D C e2 (F e1 D e2) s
   | T_DCast _ e1 C D e2 s n => f4 e1 C D e2 (F e1 D e2) s n
